improve prepost automation

theories/Ref/Automation.v
@@ -1,6 +1,7 @@
 From Coq Require Export
      Datatypes
      Arith.PeanoNat
+     Wf_nat
      Morphisms
      Setoid
      Program.Equality
@@ -927,7 +928,16 @@ Ltac IntroArg_forget := let e := fresh in intro e; clear e.
 Polymorphic Lemma IntroArg_beta n A (f : A -> Type) x goal :
   IntroArg n (f x) goal ->
   IntroArg n ((fun x' => f x') x) goal.
-Proof. eauto. Qed.
+Proof. eauto. Defined.
+
+Polymorphic Lemma IntroArg_sigT n A P (goal : sigT P -> Type)
+  : IntroArg n A (fun a => IntroArg n (P a) (fun p => goal (existT _ a p))) ->
+    IntroArg n _ goal.
+Proof. intros H []; apply H. Defined.
+
+Polymorphic Lemma IntroArg_unit n (goal : unit -> Type)
+  : goal tt -> IntroArg n _ goal.
+Proof. intros H []; apply H. Defined.
 
 Polymorphic Lemma IntroArg_and n P Q (goal : P /\ Q -> Prop)
   : IntroArg n P (fun p => IntroArg n Q (fun q => goal (conj p q))) ->
@@ -1062,6 +1072,8 @@ Ltac IntroArg_intro_dependent_destruction n :=
 Ltac IntroArg_base_tac n A g :=
   lazymatch A with
   | (fun _ => _) _ => simple apply IntroArg_beta
+  | sigT _ => simple apply IntroArg_sigT
+  | unit => simple apply IntroArg_unit
   | _ /\ _ => simple apply IntroArg_and
   | True => simple apply IntroArg_true
   | False => simple apply IntroArg_false
@@ -1098,7 +1110,7 @@ Ltac IntroArg_base_tac n A g :=
   apply (@IntroArg_FrameCall n frame) : refines.
 #[global] Hint Extern 101 (IntroArg ?n (LRTInput _) _) =>
   apply IntroArg_LRTInput_Fun || apply IntroArg_LRTInput_Ret;
-  simpl lrtApply; simpl applyFrameTuple : refines.
+  simpl lrtApply; simpl applyFrameTuple : refines prepostcond.
   
 #[global] Hint Extern 102 (IntroArg ?n (@eq bool _ _) _) =>
   let e := argName n in IntroArg_intro e; rewrite e in * : refines prepostcond.
@@ -1474,24 +1486,32 @@ Hint Extern 101 (spec_refines _ _ _ ((match _ with | (_,_) => _ end) >>= _) _) =
 Definition PreAndPostConditions frame1 frame2 : Type :=
   Rel (FrameCall frame1) (FrameCall frame2) *
   PostRel (FrameCall frame1) (FrameCall frame2).
+
 Definition WellFoundedRelationOn {A} (_ _ : A) := Prop.
 Definition WellFoundedRelation A :=
   IntroArg Any A (fun a1 => IntroArg Any A (fun a2 =>
-    WellFoundedRelationOn a1 a2)).  
+    WellFoundedRelationOn a1 a2)).
 
 #[global] Hint Extern 101 (WellFoundedRelation _) =>
   unfold WellFoundedRelation : prepostcond.
+
+#[global] Hint Extern 101 (well_founded (fun _ _ => False)) =>
+  constructor; contradiction : refines prepostcond.
+#[global] Hint Extern 101 (well_founded (fun _ _ => _ < _)) =>
+  apply well_founded_ltof : refines prepostcond.
+#[global] Hint Extern 101 (well_founded (fun _ _ => _ > _)) =>
+  apply well_founded_gtof : refines prepostcond.
 
 Inductive ContinueType := Continue_multifix | Continue_total_spec.
 Polymorphic Definition ContinueArg ct : Type :=
   match ct with
   | Continue_multifix => (Prop * Type * Type)%type
-  | Continue_total_spec => (Prop * Prop * Type * Type)%type
+  | Continue_total_spec => (Prop * Prop * Prop * Type * Type)%type
   end.
 Polymorphic Definition Continue {ct : ContinueType} : ContinueArg ct -> Type :=
-  match ct with
+  match ct return ContinueArg ct -> Type with
   | Continue_multifix => fun '(precond, goal1, goal2) => (precond * goal1 * goal2)%type
-  | Continue_total_spec => fun '(tsPre, precond, H, goal) => (tsPre * precond * H * goal)%type
+  | Continue_total_spec => fun '(wf, tsPre, precond, H, goal) => (wf * tsPre * precond * H * goal)%type
   end.
 Arguments Continue {ct carg}.
 
@@ -1499,9 +1519,9 @@ Lemma Continue_multifix_unfold precond goal1 goal2 :
   RelGoal precond -> goal1 -> goal2 ->
   @Continue Continue_multifix (precond, goal1, goal2).
   Proof. split; eauto. Qed.
-Lemma Continue_total_spec_unfold tsPre precond H goal :
-  RelGoal tsPre -> RelGoal precond -> H -> goal ->
-  @Continue Continue_total_spec (tsPre, precond, H, goal).
+Lemma Continue_total_spec_unfold wf tsPre precond H goal :
+  RelGoal wf -> RelGoal tsPre -> RelGoal precond -> H -> goal ->
+  @Continue Continue_total_spec (wf, tsPre, precond, H, goal).
 Proof. split; eauto. Qed.
 
 Ltac Continue_unfold :=
@@ -1586,9 +1606,9 @@ Lemma spec_refines_total_spec_IntroArg (E1 E2 : EvType) Γ1 Γ2 frame1
       (tsPre : A2 -> Prop) (tsPost : A2 -> B2 -> Prop)
       (rdec : WellFoundedRelation A2)
       (prepostconds : PreAndPostConditions frame1 (unary1Frame A2 B2)) :
-  well_founded rdec ->
   @Continue Continue_total_spec
-            (tsPre a2, fst prepostconds call1 (unary1Call a2),
+            (well_founded rdec,
+             tsPre a2, fst prepostconds call1 (unary1Call a2),
              IntroArg RetAny _ (fun r1 => IntroArg RetAny _ (fun r2 =>
               IntroArg Hyp (tsPost a2 r2) (fun _ =>
               IntroArg Hyp (snd prepostconds call1 (unary1Call a2) r1 r2) (fun _ =>
@@ -1606,7 +1626,7 @@ Lemma spec_refines_total_spec_IntroArg (E1 E2 : EvType) Γ1 Γ2 frame1
                (MultiFixS E1 Γ1 frame1 bodies1 call1)
                (total_spec tsPre tsPost a2).
 Proof.
-  destruct prepostconds; intros ? [[[]]].
+  destruct prepostconds; intros [[[[]]]].
   unfold IntroArg, RelGoal in *; simpl in *.
   unshelve eapply spec_refines_total_spec; eauto.
 Qed.
@@ -1678,16 +1698,49 @@ Hint Extern 992 (spec_refines _ _ _ _ (trepeat _ _ >>= _)) =>
   simple apply spec_refines_trepeat_bind_zero_r : refines.
 
 
+(** * Tactics for proving refinement *)
+
+Ltac prove_refinement_eauto :=
+  unshelve (typeclasses eauto with refines).
+
+Ltac prove_refinement_prepostcond :=
+  try (unshelve (typeclasses eauto with prepostcond)).
+
+Ltac prove_refinement :=
+  prove_refinement_eauto; prove_refinement_prepostcond;
+  try reflexivity || contradiction.
+
+Ltac prove_refinement_continue :=
+  Continue_unfold; prove_refinement.
+
+
 (** * Tactics for building pre/post-conditions *)
 
+Definition PreCase {frame1 frame2} i j
+  (a1 : LRTInput (nthLRT frame1 i))
+  (a2 : LRTInput (nthLRT frame2 j)) := Prop.
+Definition PostCase {frame1 frame2} i j args1 args2
+  (r1 : LRTOutput (nthLRT frame1 i) args1)
+  (r2 : LRTOutput (nthLRT frame2 j) args2) := Prop.
+
+#[global] Hint Opaque PreCase : prepostcond.
+#[global] Hint Opaque PostCase : prepostcond.
+
+#[global] Hint Extern 999 (PreCase _ _ _ _) => shelve : prepostcond.
+#[global] Hint Extern 999 (PostCase _ _ _ _ _ _) => shelve : prepostcond.
+
 Definition prepost_case {frame1 frame2} i j
-  (pre : Rel (LRTInput (nthLRT frame1 i)) (LRTInput (nthLRT frame2 j)))
-  (post : forall args1 args2, Rel (LRTOutput (nthLRT frame1 i) args1)
-                                  (LRTOutput (nthLRT frame2 j) args2))
+  (pre : IntroArg Any (LRTInput (nthLRT frame1 i)) (fun a1 =>
+         IntroArg Any (LRTInput (nthLRT frame2 j)) (fun a2 =>
+         PreCase i j a1 a2)))
+  (post : IntroArg Any _ (fun args1 => IntroArg Any _ (fun args2 =>
+          IntroArg RetAny (LRTOutput (nthLRT frame1 i) args1) (fun r1 =>
+          IntroArg RetAny (LRTOutput (nthLRT frame2 j) args2) (fun r2 =>
+          PostCase i j args1 args2 r1 r2)))))
   (prepostcond : PreAndPostConditions frame1 frame2) :
   PreAndPostConditions frame1 frame2.
 Proof.
-  split.
+  unfold IntroArg, PreCase, PostCase in *; split.
   all: intros [m args1] [n args2].
   all: destruct (Nat.eq_dec m i) as [p1|]; destruct (Nat.eq_dec n j) as [p2|].
   all: try (destruct p1; destruct p2).
@@ -1709,11 +1762,11 @@ Notation eqPostCase :=
   (only parsing).
 
 Tactic Notation "prepost_case" constr(i) constr(j) :=
-  apply (prepost_case i j).
+  apply (prepost_case i j); prove_refinement_prepostcond.
 Tactic Notation "prepost_case" constr(i) constr(j) "withPre" uconstr(pre) :=
-  apply (prepost_case i j); [ exact pre | |].
+  apply (prepost_case i j); [ exact pre | prove_refinement_prepostcond |].
 Tactic Notation "prepost_case" constr(i) constr(j) "withPost" uconstr(post) :=
-  apply (prepost_case i j); [| exact post |].
+  apply (prepost_case i j); [ prove_refinement_prepostcond | exact post |].
 Tactic Notation "prepost_case" constr(i) constr(j) "with" uconstr(pre) "," uconstr(post) :=
   apply (prepost_case i j); [exact pre | exact post |].
 
@@ -1733,21 +1786,6 @@ Tactic Notation "prepost_exclude_remaining" :=
 #[global] Hint Extern 101 (RelGoal (snd (prepost_case _ _ _ _ _) _ _ _ _)) =>
   unfold RelGoal; simpl; apply RelGoal_fold : refines.
 
-
-(** * Tactics for proving refinement *)
-
-Ltac prove_refinement_eauto :=
-  unshelve (typeclasses eauto with refines).
-
-Ltac prove_refinement_prepostcond :=
-  try (unshelve (typeclasses eauto with prepostcond)).
-
-Ltac prove_refinement :=
-  prove_refinement_eauto; prove_refinement_prepostcond;
-  try reflexivity || contradiction.
-
-Ltac prove_refinement_continue :=
-  Continue_unfold; prove_refinement.
 
 
 (** * Testing *)
@@ -1816,10 +1854,8 @@ Lemma test_total_spec_easy E (x : nat) :
 Proof.
   prove_refinement.
   - exact False.
-  - prepost_case 0 0 withPre eqPreCase.
-    { simpl. intros [] [] r1 r2. exact (r1 = r2). }
+  - prepost_case 0 0 withPre eqPreCase; [ exact (r = r0) |].
     prepost_exclude_remaining.
-  - constructor; contradiction.
   - prove_refinement_continue.
 Qed.
 
